Low/Reduce_by_P_compose.v
@@ -1,0 +1,494 @@
+From Tweetnacl Require Import Libs.Export.
+From Tweetnacl Require Import ListsOp.Export.
+(* From Tweetnacl Require Import Mid.SubList. *)
+(* From Tweetnacl Require Import Low.Get_abcdef. *)
+(* From Tweetnacl Require Import Low.GetBit_pack25519. *)
+(* From Tweetnacl Require Import Low.Sel25519. *)
+(* From Tweetnacl Require Import Low.Constant. *)
+From stdpp Require Import prelude.
+Require Import Recdef.
+
+(*
+sv pack25519(u8 *o,const gf n)
+{
+  int i,j,b;
+  gf m,t;
+  FOR(i,16) t[i]=n[i];
+  car25519(t);
+  car25519(t);
+  car25519(t);
+  FOR(j,2) {
+    m[0]=t[0]-0xffed;
+
+    for(i=1;i<15;i++) {
+      m[i]=t[i]-0xffff-((m[i-1]>>16)&1);
+      m[i-1]&=0xffff;
+    }
+
+    m[15]=t[15]-0x7fff-((m[14]>>16)&1);
+    b=(m[15]>>16)&1;
+    m[14]&=0xffff;
+    sel25519(t,m,1-b);
+  }
+  FOR(i,16) {
+    o[2*i]=t[i]&0xff;
+    o[2*i+1]=t[i]>>8;
+  }
+}
+*)
+
+Open Scope Z.
+(*
+0xffff = 65535
+0xffed = 65517
+0x7fff = 32767
+*)
+
+Definition subst_0xffed t := t - 65517.
+Definition subst_0xffffc t m := t - 65535 - (Z.land (Z.shiftr m 16) 1).
+Definition subst_0xffff t := t - 65535.
+Definition subst_0x7fffc t m := t - 32767 - (Z.land (Z.shiftr m 16) 1).
+Definition subst_0x7fff t := t - 32767.
+Definition subst_c t m := t - (Z.land (Z.shiftr m 16) 1).
+Definition mod0xffff m := Z.land m 65535.
+
+Definition sub_step (a:Z) (m t:list Z) : list Z :=
+    let m' := nth (Z.to_nat (a - 1)) m 0 in
+    let t' := nth (Z.to_nat a) t 0 in
+      upd_nth (Z.to_nat (a-1)) (upd_nth (Z.to_nat a) m (subst_0xffffc t' m')) (mod0xffff m').
+
+Lemma nth_i_1_substep: forall i m t, 
+  Zlength m = Zlength t ->
+  0 < i < Zlength m ->
+  nth (Z.to_nat (i - 1)) (sub_step i m t) 0 = mod0xffff (nth (Z.to_nat (i - 1)) m 0).
+Proof.
+  intros i m t Hmt Him.
+  rewrite /sub_step /mod0xffff.
+  rewrite upd_nth_same_Zlength ; try reflexivity.
+  split ; try omega ; rewrite upd_nth_Zlength ; rewrite Z2Nat.id ; try omega.
+Qed.
+
+Lemma nth_i_substep: forall i m t, 
+  Zlength m = Zlength t ->
+  0 < i < Zlength m ->
+  nth (Z.to_nat (i)) (sub_step i m t) 0 = subst_0xffffc (nth (Z.to_nat i) t 0) (nth (Z.to_nat (i - 1)) m 0).
+Proof.
+  intros i m t Hmt Him.
+  rewrite /sub_step.
+  rewrite upd_nth_diff_Zlength.
+  2: split ; try omega ; rewrite upd_nth_Zlength ; rewrite Z2Nat.id ; try omega.
+  2: split ; try omega ; rewrite upd_nth_Zlength ; rewrite Z2Nat.id ; try omega.
+  2: intros H ; apply (f_equal Z.of_nat) in H ; rewrite ?Z2Nat.id in H ; omega.
+  rewrite upd_nth_same_Zlength ; try reflexivity.
+  rewrite Z2Nat.id ; try omega.
+Qed.
+
+Definition sub_step_1 (a:Z) (m t:list Z) : list Z :=
+    let t' := nth (Z.to_nat a) t 0 in
+      (upd_nth (Z.to_nat a) m (subst_0xffff t')).
+
+Definition sub_step_2 (a:Z) (m:list Z) : list Z :=
+    let m' := nth (Z.to_nat (a - 1)) m 0 in
+    let t' := nth (Z.to_nat a) m 0 in
+      upd_nth (Z.to_nat (a-1)) (upd_nth (Z.to_nat a) m (subst_c t' m')) (mod0xffff m').
+
+Lemma subst_step_1_2 : forall a m t,
+  0 < a < Zlength m ->
+  sub_step a m t = sub_step_2 a (sub_step_1 a m t).
+Proof.
+  intros.
+  rewrite /sub_step /sub_step_1 /sub_step_2 /subst_0xffff /mod0xffff /subst_0xffffc.
+  rewrite ?upd_nth_same_Zlength.
+  rewrite ?upd_nth_diff_Zlength.
+  f_equal.
+  rewrite upd_nth_upd_nth_Zlength.
+  reflexivity.
+  all: try (rewrite Z2Nat.id ; omega).
+  clear t.
+  intro Ha.
+  apply (f_equal Z.of_nat) in Ha.
+  rewrite ?Z2Nat.id in Ha ; omega.
+Qed.
+
+(* Definition of the for loop : 1 -> 15 *)
+Function sub_fn_rev {A} (f:Z -> list A -> list A -> list A) (a:Z) (m t: list A) {measure Z.to_nat a} : (list A) :=
+  if (a <=? 1)
+    then m
+    else
+      let prev := sub_fn_rev f (a - 1) m t in 
+        f (a - 1) prev t.
+Proof. intros. apply Z2Nat.inj_lt ; move: teq ; rewrite Z.leb_gt => teq; omega. Defined.
+
+Arguments sub_fn_rev [_] _ _ _.
+
+Lemma sub_fn_rev_1 : forall A f (m t:list A),
+  sub_fn_rev f 1 m t = m.
+Proof. go. Qed.
+
+Lemma sub_fn_rev_n : forall A f (m t:list A) a,
+  1 < a ->
+  sub_fn_rev f a m t = f (a - 1) (sub_fn_rev f (a - 1) m t) t.
+Proof. intros. rewrite sub_fn_rev_equation.
+flatten ; apply Zle_bool_imp_le in Eq; omega.
+Qed.
+
+(* Definition of the for loop : 1 -> 15 *)
+Function sub_fn_rev_s {A} (f:Z -> list A -> list A) (a:Z) (m: list A) {measure Z.to_nat a} : (list A) :=
+  if (a <=? 1)
+    then m
+    else
+      let prev := sub_fn_rev_s f (a - 1) m in 
+        f (a - 1) prev.
+Proof. intros. apply Z2Nat.inj_lt ; move: teq ; rewrite Z.leb_gt => teq; omega. Defined.
+
+Arguments sub_fn_rev_s [_] _ _ _.
+
+Lemma sub_fn_rev_s_1 : forall A f (m: list A),
+  sub_fn_rev_s f 1 m = m.
+Proof. go. Qed.
+
+Lemma sub_fn_rev_s_n : forall A a (m: list A) f,
+  1 < a ->
+  sub_fn_rev_s f a m = f (a - 1) (sub_fn_rev_s f (a - 1) m).
+Proof. intros. rewrite sub_fn_rev_s_equation.
+flatten ; apply Zle_bool_imp_le in Eq; omega.
+Qed.
+
+Lemma sub_fn_rev_f_g :  forall a m t,
+  (length m = 16)%nat ->
+  (length t = 16)%nat ->
+  0 < a < 16 ->
+  sub_fn_rev sub_step a m t = sub_fn_rev_s sub_step_2 a (sub_fn_rev sub_step_1 a m t).
+Proof.
+intros a m t Hm Ht Ha.
+intros.
+do 17 (destruct m ; [tryfalse |]) ; [|tryfalse].
+do 17 (destruct t ; [tryfalse |]) ; [|tryfalse].
+assert_gen_hyp_ H a 15 14 ; try omega.
+Admitted.
+
+(*****************************************************************************************
+ *   DEFINE SEMANTIC
+ *)
+
+Inductive red_expr :=
+  | R_red : term -> red_expr
+  | Sub_red : red_expr -> red_expr
+  | SubC_red : red_expr -> red_expr -> red_expr
+  | Mod_red : red_expr -> red_expr.
+
+Inductive formula_red_expr := 
+  | Eq_red : list red_expr -> list red_expr -> formula_red_expr.
+
+Fixpoint red_expr_denote env (m : red_expr) : Z :=
+  match m with
+  | R_red  v  => term_denote env v
+  | Sub_red x => subst_0xffff (red_expr_denote env x)
+  | SubC_red x y => subst_c (red_expr_denote env x) (red_expr_denote env y)
+  | Mod_red x => mod0xffff (red_expr_denote env x)
+  end.
+
+Fixpoint red_expr_list_denote env (m: list red_expr) : list Z :=
+  match m with
+  | nil => nil
+  | h :: q => (red_expr_denote env h) :: red_expr_list_denote env q
+  end.
+
+Lemma red_expr_list_denote_nth :
+  forall i env l, red_expr_denote env (nth i l (R_red (Val 0))) = nth i (red_expr_list_denote env l) 0.
+Proof.
+intros i env l. gen i. induction l as [|h l IHl] ; intros [|i] ; try reflexivity.
+simpl. apply IHl.
+Qed.
+
+Lemma red_expr_list_denote_upd_nth :
+  forall i env l v, red_expr_list_denote env (upd_nth i l v) = upd_nth i (red_expr_list_denote env l) (red_expr_denote env v).
+Proof.
+intros i env m. gen i. induction m as [|h m IHm] ; intros [|i] v ; try reflexivity.
+simpl. f_equal. apply IHm.
+Qed.
+
+Definition formula_red_expr_denote env (t : formula_red_expr) : Prop :=
+  match t with
+  | Eq_red x y     => red_expr_list_denote env x = red_expr_list_denote env y
+  end.
+
+(*****************************************************************************************
+ *   DECIDE EQUALITY
+ *)
+
+Fixpoint decide_red_expr_eq (l1 l2:red_expr) := match l1, l2 with
+  | R_red v1 , R_red v2 => term_eqb v1 v2
+  | Sub_red v1, Sub_red v'1 => (decide_red_expr_eq v1 v'1)
+  | SubC_red v1 v2, SubC_red v'1 v'2 => andb (decide_red_expr_eq v1 v'1) (decide_red_expr_eq v2 v'2)
+  | Mod_red v1, Mod_red v2 => decide_red_expr_eq v1 v2
+  | _, _ => false
+  end.
+
+Fixpoint decide_red_expr_list_eq (l1 l2:list red_expr) := match l1, l2 with
+  | nil, nil => true
+  | h1 :: q1, h2 :: q2 => andb (decide_red_expr_eq h1 h2) (decide_red_expr_list_eq q1 q2)
+  | _, _ => false
+end.
+
+Lemma decide_red_expr_eq_impl:
+  forall env l l', 
+  decide_red_expr_eq l l' = true ->
+  red_expr_denote env l = red_expr_denote env l'.
+Proof.
+intros env.
+induction l; intros [] H ; simpl in * ;
+repeat match goal with
+  | _ => discriminate
+  | _ => reflexivity
+  | [ H : _ && _ = true |- _ ] => apply andb_prop in H; destruct H
+  | [ H : term_eqb _ _ = true |- _ ] => apply term_eqb_refl in H; subst
+  | [ H : _ = _ |- _ ] => rewrite H
+  | [ H : _ , H1 : _ |- _ ] => apply H in H1 (* why bother ? :D *)
+end.
+Qed.
+
+Lemma decide_red_expr_list_eq_impl:
+  forall env l l',
+  decide_red_expr_list_eq l l' = true ->
+  red_expr_list_denote env l = red_expr_list_denote env l'.
+Proof.
+intros env.
+induction l ; destruct l' ; intros ; simpl in *; 
+repeat match goal with
+  | _ => discriminate
+  | _ => reflexivity
+  | [ H : _ && _ = true |- _ ] => apply andb_prop in H; destruct H
+  | [ H : _ , H1 : _ |- _ ] => apply H in H1 (* why bother ? :D *)
+  | [ env: environment, H : decide_red_expr_eq _ _  = true |- _ ] => apply (decide_red_expr_eq_impl env) in H
+  | [ H : _ = _ |- _ ] => rewrite H
+  | [ H : False |- _ ] => destruct H
+end.
+Qed.
+
+Definition decide_formula_red_expr (f : formula_red_expr) : bool := match f with
+  | Eq_red x y => decide_red_expr_list_eq x y
+  end.
+
+Lemma decide_formula_red_impl : forall env f, decide_formula_red_expr f = true -> formula_red_expr_denote env f.
+Proof. move=> env [? ?]. by apply decide_red_expr_list_eq_impl. Qed.
+
+(* Weaponize our expression so we can translate functions *)
+
+Definition sub_red_step (a:Z) (m t:list red_expr) : list red_expr :=
+    let m' := nth (Z.to_nat (a - 1)) m (R_red (Val 0)) in
+    let t' := nth (Z.to_nat a) t (R_red (Val 0)) in
+      upd_nth (Z.to_nat (a-1)) (upd_nth (Z.to_nat a) m (SubC_red (Sub_red t') m')) (Mod_red m').
+
+Definition sub_red_step_1 (a:Z) (m t:list red_expr) : list red_expr :=
+    let t' := nth (Z.to_nat a) t (R_red (Val 0)) in
+      (upd_nth (Z.to_nat a) m (Sub_red t')).
+
+Definition sub_red_step_2 (a:Z) (m:list red_expr) : list red_expr :=
+    let m' := nth (Z.to_nat (a - 1)) m (R_red (Val 0)) in
+    let t' := nth (Z.to_nat a) m (R_red (Val 0)) in
+      upd_nth (Z.to_nat (a-1)) (upd_nth (Z.to_nat a) m (SubC_red t' m')) (Mod_red m').
+
+Lemma step_fn_red_expr : forall env a m t,
+  sub_fn_rev sub_step a (red_expr_list_denote env m) (red_expr_list_denote env t) =
+  red_expr_list_denote env (sub_fn_rev sub_red_step a m t).
+Proof.
+intros env [ | p | p] m t.
+all: try reflexivity.
+assert(Hi:= Pos2Z.is_nonneg p).
+remember (Z.pos p) as i.
+clears p.
+gen m t.
+apply (natlike_ind (fun i => ∀ m t : list red_expr,
+sub_fn_rev sub_step i (red_expr_list_denote env m) (red_expr_list_denote env t) =
+red_expr_list_denote env (sub_fn_rev sub_red_step i m t))) ; try omega.
+intros ; reflexivity.
+clears i.
+intros i Hi IH m t.
+assert(Hii: i = 0 \/ 0 < i) by omega.
+change (Z.succ i) with (i + 1).
+destruct Hii as [Hii|Hii] ; try (subst i ; reflexivity).
+rewrite sub_fn_rev_n.
+symmetry.
+rewrite sub_fn_rev_n.
+symmetry.
+replace (i + 1 - 1) with i.
+all: try omega.
+rewrite /sub_red_step.
+rewrite ?red_expr_list_denote_upd_nth.
+rewrite /sub_step.
+rewrite ?red_expr_list_denote_nth. simpl.
+rewrite /subst_0xffffc /subst_c /subst_0xffff.
+rewrite IH.
+rewrite ?red_expr_list_denote_nth.
+reflexivity.
+Qed.
+
+Lemma step_fn_red_expr_1 : forall env a m t,
+  sub_fn_rev sub_step_1 a (red_expr_list_denote env m) (red_expr_list_denote env t) =
+  red_expr_list_denote env (sub_fn_rev sub_red_step_1 a m t).
+Proof.
+intros env [ | p | p] m t.
+all: try reflexivity.
+assert(Hi:= Pos2Z.is_nonneg p).
+remember (Z.pos p) as i.
+clears p.
+gen m t.
+apply (natlike_ind (fun i => ∀ m t : list red_expr,
+sub_fn_rev sub_step_1 i (red_expr_list_denote env m) (red_expr_list_denote env t) =
+red_expr_list_denote env (sub_fn_rev sub_red_step_1 i m t))) ; try omega.
+intros ; reflexivity.
+clears i.
+intros i Hi IH m t.
+assert(Hii: i = 0 \/ 0 < i) by omega.
+change (Z.succ i) with (i + 1).
+destruct Hii as [Hii|Hii] ; try (subst i ; reflexivity).
+rewrite sub_fn_rev_n.
+symmetry.
+rewrite sub_fn_rev_n.
+symmetry.
+replace (i + 1 - 1) with i.
+all: try omega.
+rewrite /sub_red_step.
+rewrite ?red_expr_list_denote_upd_nth.
+rewrite /sub_step.
+rewrite ?red_expr_list_denote_nth. simpl.
+rewrite /subst_0xffffc /subst_c /subst_0xffff.
+rewrite IH.
+rewrite ?red_expr_list_denote_nth.
+reflexivity.
+Qed.
+
+Lemma step_fn_red_expr_2 : forall env a m,
+  sub_fn_rev_s sub_step_2 a (red_expr_list_denote env m) =
+  red_expr_list_denote env (sub_fn_rev_s sub_red_step_2 a m).
+Proof.
+intros env [ | p | p] m.
+all: try reflexivity.
+assert(Hi:= Pos2Z.is_nonneg p).
+remember (Z.pos p) as i.
+clears p.
+gen m.
+apply (natlike_ind (fun i => ∀ m : list red_expr,
+sub_fn_rev_s sub_step_2 i (red_expr_list_denote env m) =
+red_expr_list_denote env (sub_fn_rev_s sub_red_step_2 i m))) ; try omega.
+intros ; reflexivity.
+clears i.
+intros i Hi IH m.
+assert(Hii: i = 0 \/ 0 < i) by omega.
+change (Z.succ i) with (i + 1).
+destruct Hii as [Hii|Hii] ; try (subst i ; reflexivity).
+rewrite sub_fn_rev_s_n.
+symmetry.
+rewrite sub_fn_rev_s_n.
+symmetry.
+replace (i + 1 - 1) with i.
+all: try omega.
+rewrite /sub_red_step.
+rewrite ?red_expr_list_denote_upd_nth.
+rewrite /sub_step.
+rewrite ?red_expr_list_denote_nth. simpl.
+rewrite /subst_0xffffc /subst_c /subst_0xffff.
+rewrite IH.
+rewrite ?red_expr_list_denote_nth.
+reflexivity.
+Qed.
+
+Close Scope Z.
+
+
+(**************************************************************************
+ * Reflection tactics
+ *)
+
+(*
+Ltac reifyValue env t :=
+  match t with
+  | ?X =>
+    let v := lookup X env in
+    constr:(R_inv)
+  | _ => constr:(R_inv)
+  end.
+
+Ltac reifyExpr env t :=
+  lazymatch t with
+  | pow_fn_rev_Z ?a ?b ?X ?Y =>
+    let x := reifyValue env X in
+    let y := reifyValue env Y in
+    constr:(pow_inv (Z.to_nat a) (Z.to_nat b) x y)
+  | ?X * ?Y =>
+    let x := reifyValue env X in
+    let y := reifyValue env Y in
+    constr:(M_inv x y)
+  | Z.pow ?X ?Y =>
+    let x := reifyValue env X in
+    match Y with
+      | Z.pos ?p => constr:(P_inv x p)
+      | _ => constr:(P_inv x 1%positive)
+    end
+  | ?X =>
+    let x := reifyValue env X in
+    constr:(R_inv)
+  end.
+
+Ltac reifyTerm env t :=
+  lazymatch t with
+   | ?X = ?Y =>
+      let x := reifyExpr env X in
+      let y := reifyExpr env Y in
+      constr:(Eq_inv x y)
+  end.
+
+Ltac functionalize xs :=
+  let rec loop n xs' :=
+    lazymatch xs' with
+    | tt => constr:(fun _ : positive => 0%Z)
+    | (?x, tt) => constr:(fun _ : positive => x)
+    | (?x, ?xs'') =>
+      let f := loop (Pos.succ n) xs'' in
+      constr:(fun m : positive => if (m =? n)%positive then x else f m)
+    end in
+  loop (1%positive) xs.
+
+(**************************************************************************
+ * User interface tactics
+ *)
+
+Open Scope Z.
+(* 
+Eval compute in Z.pow 2 255 - 21.
+Z.pow 2 255 - 21 = 57896044618658097711785492504343953926634992332820282019728792003956564819947
+*)
+
+Theorem Inv25519_Z_correct : forall x, Inv25519_Z x = Z.pow x 57896044618658097711785492504343953926634992332820282019728792003956564819947.
+Proof.
+intros.
+  rewrite /Inv25519_Z.
+  match goal with
+  | [ |- ?X ] =>
+    let xss := constr:((x, tt)) in
+    let envv := functionalize xss in
+    let r1  := reifyTerm xss X in
+    pose xs := xss;
+    pose env := envv;
+    pose reif := r1
+    end.
+    (* in theory we would use change, but here we need to proceed slightly differently *)
+    assert (
+      formula_inv_denote (Var 1) {| vars := env |} reif ->
+      pow_fn_rev_Z 254 254 x x =
+      x ^ 57896044618658097711785492504343953926634992332820282019728792003956564819947).
+    {
+    subst env reif.
+    rewrite /formula_inv_denote pow_inv_pow_fn_rev_eq.
+    simpl. trivial.
+    }
+    apply H ; clear H.
+    apply decide_formula_inv_impl.
+    (* at this point we don't need any hypothesis, this is purely computational *)
+    subst reif ; clears.
+    compute.
+    reflexivity.
+Qed.
+
+Close Scope Z. *)
